WIP

Definitions.v
@@ -4,6 +4,561 @@
  ************************************************)
 
 Set Implicit Arguments.
-Require Import LibLN.
+Require Import List LibLN.
 Implicit Types x : var.
 Implicit Types X : var.
+
+(* *************************************************************** *)
+(** ** Description of types *)
+
+(* Kinds *)
+Inductive kind : Set :=
+  | kind_type : kind
+  | kind_row : kind.
+
+(** Representation of pre-types *)
+
+Inductive typ : Set :=
+  | typ_bvar : nat -> typ
+  | typ_fvar : var -> typ
+  | typ_constructor : nat -> typ -> typ
+  | typ_variant : typ -> typ -> typ
+  | typ_arrow : typ -> typ -> typ
+  | typ_top : typ
+  | typ_bot : typ
+  | typ_meet : typ -> typ -> typ
+  | typ_join : typ -> typ -> typ.
+
+(** Types are inhabited, giving us a default value. *)
+
+Definition typ_def := typ_bvar 0.
+
+(** Type schemes. *)
+
+Record sch : Set := Sch { 
+  sch_kinds : list kind ;
+  sch_type  : typ }.
+
+Definition sch_arity M := length (sch_kinds M).
+
+(** Opening body of type schemes. *)
+
+Fixpoint typ_open (T : typ) (Vs : list typ) {struct T} : typ :=
+  match T with
+  | typ_bvar i => nth i Vs typ_def
+  | typ_fvar x => typ_fvar x 
+  | typ_constructor c T => typ_constructor c (typ_open T Vs)
+  | typ_variant T1 T2 => typ_variant (typ_open T1 Vs) (typ_open T2 Vs)
+  | typ_arrow T1 T2 => typ_arrow (typ_open T1 Vs) (typ_open T2 Vs)
+  | typ_top => typ_top
+  | typ_bot => typ_bot
+  | typ_meet T1 T2 => typ_meet (typ_open T1 Vs) (typ_open T2 Vs)
+  | typ_join T1 T2 => typ_join (typ_open T1 Vs) (typ_open T2 Vs)
+  end.
+
+(** Opening body of type schemes with variables *)
+
+Definition typ_fvars := 
+  List.map typ_fvar.
+
+Definition typ_open_vars T Xs := 
+  typ_open T (typ_fvars Xs).
+
+(** Instanciation of a type scheme *)
+
+Definition sch_open M := 
+  typ_open (sch_type M).
+
+Definition sch_open_vars M := 
+  typ_open_vars (sch_type M).
+
+Notation "M ^^ Vs" := (sch_open M Vs) 
+  (at level 67, only parsing) : typ_scope.
+Notation "M ^ Xs" := 
+  (sch_open_vars M Xs) (only parsing) : typ_scope.
+
+Bind Scope typ_scope with typ.
+Open Scope typ_scope.
+
+(** Locally closed types *)
+
+Inductive type : typ -> Prop :=
+  | type_fvar : forall X, 
+      type (typ_fvar X)
+  | type_constructor : forall c T,
+      type T ->
+      type (typ_constructor c T)
+  | type_variant : forall T1 T2,
+      type T1 ->
+      type T2 ->
+      type (typ_variant T1 T2)
+  | type_arrow : forall T1 T2,
+      type T1 -> 
+      type T2 -> 
+      type (typ_arrow T1 T2)
+  | type_top : type (typ_top)
+  | type_bot : type (typ_bot)
+  | type_meet : forall T1 T2,
+      type T1 ->
+      type T2 ->
+      type (typ_meet T1 T2)
+  | type_join : forall T1 T2,
+      type T1 ->
+      type T2 ->
+      type (typ_join T1 T2).
+
+(** List of n locally closed types *)
+
+Definition types n (L : list typ) :=
+  n = length L /\ Forall type L.
+
+(** Body of a scheme *)
+
+Definition type_body n T :=
+  exists L, forall Xs,
+  fresh L n Xs ->
+  type (typ_open_vars T Xs).
+
+(** Definition of a well-formed scheme *)
+
+Definition scheme M :=
+  type_body (sch_arity M) (sch_type M).
+
+(* ************************************************************** *)
+(** ** Description of terms *)
+
+(** Representation of pre-terms *)
+
+Inductive trm : Set :=
+  | trm_bvar : nat -> trm
+  | trm_fvar : var -> trm
+  | trm_abs : trm -> trm
+  | trm_let : trm -> trm -> trm
+  | trm_app : trm -> trm -> trm
+  | trm_constructor : nat -> trm -> trm
+  | trm_match : trm -> nat -> trm -> trm -> trm
+  | trm_absurd : trm -> trm.
+
+Fixpoint trm_open_rec (k : nat) (u : trm) (t : trm) {struct t} : trm :=
+  match t with
+  | trm_bvar i => If k = i then u else (trm_bvar i)
+  | trm_fvar x => trm_fvar x 
+  | trm_abs t1 => trm_abs (trm_open_rec (S k) u t1) 
+  | trm_let t1 t2 =>
+      trm_let (trm_open_rec k u t1) (trm_open_rec (S k) u t2) 
+  | trm_app t1 t2 =>
+      trm_app (trm_open_rec k u t1) (trm_open_rec k u t2)
+  | trm_constructor c t =>
+      trm_constructor c (trm_open_rec k u t)
+  | trm_match t1 c t2 t3 =>
+      trm_match (trm_open_rec k u t1) c
+                (trm_open_rec (S k) u t2)
+                (trm_open_rec (S k) u t3)
+  | trm_absurd t1 => trm_absurd (trm_open_rec k u t1)
+  end.
+
+Definition trm_open t u := trm_open_rec 0 u t.
+
+Notation "{ k ~> u } t" := (trm_open_rec k u t) (at level 67).
+Notation "t ^^ u" := (trm_open t u) (at level 67).
+Notation "t ^ x" := (trm_open t (trm_fvar x)).
+
+(** Locally closed term *)
+
+Inductive term : trm -> Prop :=
+  | term_var : forall x, 
+      term (trm_fvar x)
+  | term_abs : forall L t1,
+      (forall x, x \notin L -> term (t1 ^ x)) -> 
+      term (trm_abs t1)
+  | term_let : forall L t1 t2,
+      term t1 -> 
+      (forall x, x \notin L -> term (t2 ^ x)) -> 
+      term (trm_let t1 t2)
+  | term_app : forall t1 t2,
+      term t1 -> 
+      term t2 -> 
+      term (trm_app t1 t2)
+  | term_constructor : forall c t,
+      term t ->
+      term (trm_constructor c t)
+  | term_match : forall L t1 c t2 t3,
+      term t1 ->
+      (forall x, x \notin L -> term (t2 ^ x)) ->
+      (forall x, x \notin L -> term (t3 ^ x)) ->
+      term (trm_match t1 c t2 t3)
+  | term_absurd : forall t,
+      term t ->
+      term (trm_absurd t).
+
+
+(** Definition of the body of an abstraction *)
+
+Definition term_body t :=
+  exists L, forall x, x \notin L -> term (t ^ x).
+
+(* ************************************************************* *)
+(** ** Description of typing environments *)
+
+(** A binding is either mapping type or term variables. 
+ [X ~:: T] is a kinding asumption and [x ~: T] is
+ a typing assumption *)
+
+Inductive bind : Set :=
+  | bind_kind : kind -> bind
+  | bind_typ : sch -> bind.
+
+Definition bind_kinds Xs Ks :=
+  map bind_kind (Xs ~* Ks).
+
+Notation "X ~:: K" := (X ~ bind_kind K)
+  (at level 23, left associativity) : env_scope.
+Notation "x ~: T" := (x ~ bind_typ T)
+  (at level 23, left associativity) : env_scope.
+Notation "Xs ~::* Ks" := (map bind_kind (Xs ~* Ks))
+  (at level 23, left associativity) : env_scope.
+
+(** Pre-environment is an associative list of bindings. *)
+
+Definition env := LibEnv.env bind.
+
+(** Environment is a pre-environment with unique bindings *)
+
+Inductive environment : env -> Prop :=
+  | environment_empty :
+      environment empty
+  | environment_kind : forall E X K,
+      environment E ->
+      X # E ->
+      environment (E & X ~:: K)
+  | environment_typ : forall E x M,
+      environment E ->
+      scheme M ->
+      x # E ->
+      environment (E & x ~: M).
+
+(* ************************************************************* *)
+(** ** Description of typing *)
+
+(** The kinding relation *)
+
+Inductive kinding : env -> typ -> kind -> Prop :=
+  | kinding_var : forall K E X,
+      environment E ->
+      binds X (bind_kind K) E ->
+      kinding E (typ_fvar X) K
+  | kinding_constructor : forall E c T,
+      kinding E T kind_type ->
+      kinding E (typ_constructor c T) kind_row
+  | kinding_variant : forall E T1 T2,
+      kinding E T1 kind_row ->
+      kinding E T2 kind_row ->
+      kinding E (typ_variant T1 T2) kind_type
+  | kinding_arrow : forall E T1 T2,
+      kinding E T1 kind_type -> 
+      kinding E T2 kind_type -> 
+      kinding E (typ_arrow T1 T2) kind_type
+  | kinding_top : forall E,
+      environment E ->
+      kinding E typ_top kind_row
+  | kinding_bot : forall E,
+      environment E ->
+      kinding E typ_bot kind_row
+  | kinding_meet : forall E T1 T2,
+      kinding E T1 kind_row ->
+      kinding E T2 kind_row ->
+      kinding E (typ_meet T1 T2) kind_row
+  | kinding_join : forall E T1 T2,
+      kinding E T1 kind_row ->
+      kinding E T2 kind_row ->
+      kinding E (typ_join T1 T2) kind_row.
+
+Inductive kindings : env -> nat -> list typ -> list kind -> Prop :=
+  | kindings_nil : forall E,
+      environment E ->
+      kindings E 0 nil nil
+  | kindings_cons : forall n E T K Ts Ks,
+      kinding E T K ->
+      kindings E n Ts Ks ->
+      kindings E (S n) (T :: Ts) (K :: Ks).
+
+Definition kinding_body E n Ks T :=
+  exists L, forall Xs, 
+  fresh L n Xs ->
+  kinding (E & Xs ~::* Ks) (typ_open_vars T Xs) kind_type.
+
+Definition kinding_scheme E M :=
+  kinding_body E (sch_arity M) (sch_kinds M) (sch_type M).
+
+(** A environment E is well-kinded if it contains no duplicate bindings
+  and if each type in it is well-kinded with respect to the environment
+  it is pushed on to. *)
+
+Inductive kinding_env : env -> Prop :=
+  | kinding_env_empty :
+      kinding_env empty
+  | kinding_env_kind : forall E X K,
+      kinding_env E ->
+      X # E ->
+      kinding_env (E & X ~:: K)
+  | kinding_env_typ : forall E x M,
+      kinding_env E ->
+      kinding_scheme E M ->
+      x # E ->
+      kinding_env (E & x ~: M).
+
+(* ************************************************************* *)
+(** ** Description of typing *)
+
+(** Equality relation on types *)
+
+Inductive type_equal : env -> typ -> typ -> kind -> Prop :=
+  | type_equal_var : forall E x K,
+      environment E ->
+      binds x (bind_kind K) E ->
+      type_equal E (typ_fvar x) (typ_fvar x) K
+  | type_equal_constructor : forall E c T T',
+      type_equal E T T' kind_type ->
+      type_equal E (typ_constructor c T) (typ_constructor c T') kind_row
+  | type_equal_variant : forall E T1 T1' T2 T2',
+      type_equal E T1 T1' kind_row ->
+      type_equal E T2 T2' kind_row ->
+      type_equal E (typ_variant T1 T2) (typ_variant T1' T2') kind_type
+  | type_equal_arrow : forall E T1 T1' T2 T2',
+      type_equal E T1 T1' kind_type ->
+      type_equal E T2 T2' kind_type ->
+      type_equal E (typ_arrow T1 T2) (typ_arrow T1' T2') kind_type
+  | type_equal_top : forall E,
+      environment E ->
+      type_equal E typ_top typ_top kind_row
+  | type_equal_bot : forall E,
+      environment E ->
+      type_equal E typ_bot typ_bot kind_row
+  | type_equal_meet : forall E T1 T1' T2 T2',
+      type_equal E T1 T1' kind_row ->
+      type_equal E T2 T2' kind_row -> 
+      type_equal E (typ_meet T1 T2) (typ_meet T1' T2') kind_row
+  | type_equal_join : forall E T1 T1' T2 T2',
+      type_equal E T1 T1' kind_row ->
+      type_equal E T2 T2' kind_row ->
+      type_equal E (typ_join T1 T2) (typ_join T1' T2') kind_row
+  | type_equal_trans : forall E T1 T2 T3 K,
+      type_equal E T1 T2 K ->
+      type_equal E T2 T3 K ->
+      type_equal E T1 T3 K
+  | type_equal_meet_commutative : forall E T1 T2,
+      kinding E T1 kind_row ->
+      kinding E T2 kind_row ->
+      type_equal E (typ_meet T1 T2) (typ_meet T2 T1) kind_row
+  | type_equal_meet_associative_l : forall E T1 T2 T3,
+      kinding E T1 kind_row ->
+      kinding E T2 kind_row ->
+      kinding E T3 kind_row ->
+      type_equal E (typ_meet T1 (typ_meet T2 T3))
+                 (typ_meet (typ_meet T1 T2) T3) kind_row
+  | type_equal_meet_associative_r : forall E T1 T2 T3,
+      kinding E T1 kind_row ->
+      kinding E T2 kind_row ->
+      kinding E T3 kind_row ->
+      type_equal E (typ_meet (typ_meet T1 T2) T3)
+                 (typ_meet T1 (typ_meet T2 T3)) kind_row
+  | type_equal_meet_identity_l : forall E T,
+      kinding E T kind_row ->
+      type_equal E (typ_meet T typ_top) T kind_row
+  | type_equal_meet_identity_r : forall E T,
+      kinding E T kind_row ->
+      type_equal E T (typ_meet T typ_top) kind_row
+  | type_equal_meet_absorption_l : forall E T1 T2,
+      kinding E T1 kind_row ->
+      kinding E T2 kind_row ->
+      type_equal E (typ_meet T1 (typ_join T1 T2)) T1 kind_row
+  | type_equal_meet_absorption_r : forall E T1 T2,
+      kinding E T1 kind_row ->
+      kinding E T2 kind_row ->
+      type_equal E T1 (typ_meet T1 (typ_join T1 T2)) kind_row
+  | type_equal_meet_distribution_l : forall E T1 T2 T3,
+      kinding E T1 kind_row ->
+      kinding E T2 kind_row ->
+      kinding E T3 kind_row ->
+      type_equal E (typ_meet (typ_join T1 T2) (typ_join T1 T3))
+                 (typ_join T1 (typ_meet T2 T3)) kind_row
+  | type_equal_meet_distribution_r : forall E T1 T2 T3,
+      kinding E T1 kind_row ->
+      kinding E T2 kind_row ->
+      kinding E T3 kind_row ->
+      type_equal E (typ_join T1 (typ_meet T2 T3))
+                 (typ_meet (typ_join T1 T2) (typ_join T1 T3)) kind_row
+  | type_equal_join_commutative : forall E T1 T2,
+      kinding E T1 kind_row ->
+      kinding E T2 kind_row ->
+      type_equal E (typ_join T1 T2) (typ_join T2 T1) kind_row
+  | type_equal_join_associative_l : forall E T1 T2 T3,
+      kinding E T1 kind_row ->
+      kinding E T2 kind_row ->
+      kinding E T3 kind_row ->
+      type_equal E (typ_join T1 (typ_join T2 T3))
+                 (typ_join (typ_join T1 T2) T3) kind_row
+  | type_equal_join_associative_r : forall E T1 T2 T3,
+      kinding E T1 kind_row ->
+      kinding E T2 kind_row ->
+      kinding E T3 kind_row ->
+      type_equal E (typ_join (typ_join T1 T2) T3)
+                 (typ_join T1 (typ_join T2 T3)) kind_row
+  | type_equal_join_identity_l : forall E T,
+      kinding E T kind_row ->
+      type_equal E (typ_join T typ_bot) T kind_row
+  | type_equal_join_identity_r : forall E T,
+      kinding E T kind_row ->
+      type_equal E T (typ_join T typ_bot) kind_row
+  | type_equal_join_absorption_l : forall E T1 T2,
+      kinding E T1 kind_row ->
+      kinding E T2 kind_row ->
+      type_equal E (typ_join T1 (typ_meet T1 T2)) T1 kind_row
+  | type_equal_join_absorption_r : forall E T1 T2,
+      kinding E T1 kind_row ->
+      kinding E T2 kind_row ->
+      type_equal E T1 (typ_join T1 (typ_meet T1 T2)) kind_row
+  | type_equal_join_distribution_l : forall E T1 T2 T3,
+      kinding E T1 kind_row ->
+      kinding E T2 kind_row ->
+      kinding E T3 kind_row ->
+      type_equal E (typ_join T1 (typ_meet T2 T3))
+                 (typ_meet (typ_join T1 T2) (typ_join T1 T3)) kind_row
+  | type_equal_join_distribution : forall E T1 T2 T3,
+      kinding E T1 kind_row -> 
+      kinding E T2 kind_row ->
+      kinding E T3 kind_row ->
+      type_equal E (typ_meet (typ_join T1 T2) (typ_join T1 T3))
+                 (typ_join T1 (typ_meet T2 T3)) kind_row.
+
+
+Definition subtype E T1 T2 :=
+  type_equal E T1 (typ_join T1 T2) kind_row.
+
+Inductive typing : env -> trm -> typ -> Prop :=
+  | typing_var : forall E x M Us, 
+      kinding_env E -> 
+      binds x (bind_typ M) E -> 
+      kindings E (sch_arity M) Us (sch_kinds M) ->
+      typing E (trm_fvar x) (M ^^ Us)
+  | typing_abs : forall L E T1 T2 t1, 
+      kinding E T1 kind_type ->
+      (forall x, x \notin L -> 
+        typing (E & x ~ bind_typ (Sch nil T1)) (t1 ^ x) T2) -> 
+      typing E (trm_abs t1) (typ_arrow T1 T2)
+  | typing_app : forall E S T t1 t2, 
+      typing E t1 (typ_arrow S T) ->
+      typing E t2 S ->   
+      typing E (trm_app t1 t2) T
+  | typing_let : forall M L E T2 t1 t2, 
+      (forall Xs, fresh L (sch_arity M) Xs ->
+         typing
+           (E & Xs ~::* sch_kinds M)
+           t1 (M ^ Xs)) ->
+      (forall x, x \notin L -> typing (E & x ~ (bind_typ M)) (t2 ^ x) T2) -> 
+      typing E (trm_let t1 t2) T2
+  | typing_constructor : forall c E T1 T2 T3 t,
+      typing E t T1 ->
+      subtype E (typ_constructor c T1) T2 ->
+      subtype E T2 T3 ->
+      typing E (trm_constructor c t) (typ_variant T3 T2)
+  | typing_match : forall c L E T1 T2 T3 T4 T5 T6 t1 t2 t3,
+      typing E t1 (typ_variant T1 T2) ->
+      (forall x, x \notin L -> 
+         typing (E & x ~ bind_typ (Sch nil T3)) (t2 ^ x) T4) ->
+      (forall y, y \notin L -> 
+         typing (E & y ~ bind_typ (Sch nil (typ_variant T5 T6)))
+                (t3 ^ y) T4) ->
+      subtype E T1 (typ_join (typ_constructor c T3) T6) ->
+      subtype E T2 T1 ->
+      subtype E T6 T5 ->
+      typing E (trm_match t1 c t2 t3) T4
+  | typing_absurd : forall E T1 T2 T3 t1,
+      kinding E T3 kind_type ->
+      typing E t1 (typ_variant T1 T2) ->
+      subtype E typ_bot T2 ->
+      subtype E T2 T1 ->
+      typing E (trm_absurd t1) T3.
+
+Notation "E |= t -: T" := (typing E t T) (at level 69).
+
+Definition typing_scheme E t M :=
+  exists L, forall Xs,
+    fresh L (sch_arity M) Xs ->
+    (E & Xs ~::* sch_kinds M) |= t -: (M ^ Xs).
+
+(* ************************************************************* *)
+(** ** Description of the semantics *)
+
+(** Grammar of values *)
+
+Inductive value : trm -> Prop :=
+  | value_constructor : forall c t,
+      value t -> value (trm_constructor c t)
+  | value_abs : forall t,
+      term (trm_abs t) -> value (trm_abs t).
+
+(** Reduction rules *)
+
+Inductive red : trm -> trm -> Prop :=
+  | red_let : forall t1 t2, 
+      term (trm_let t1 t2) ->
+      value t1 -> 
+      red (trm_let t1 t2) (t2 ^^ t1)
+  | red_let_1 : forall t1 t1' t2, 
+      term_body t2 ->
+      red t1 t1' -> 
+      red (trm_let t1 t2) (trm_let t1' t2)
+  | red_app_1 : forall t1 t1' t2,
+      term t2 ->
+      red t1 t1' -> 
+      red (trm_app t1 t2) (trm_app t1' t2)
+  | red_app_2 : forall t1 t2 t2', 
+      value t1 ->
+      red t2 t2' ->
+      red (trm_app t1 t2) (trm_app t1 t2')
+  | red_app_3 : forall t1 t2, 
+      term_body t1 -> 
+      value t2 ->  
+      red (trm_app (trm_abs t1) t2) (t1 ^^ t2)
+  | red_constructor : forall c t t',
+      red t t' ->
+      red (trm_constructor c t) (trm_constructor c t')
+  | red_match_1 : forall c t1 t1' t2 t3,
+      term_body t2 ->
+      term_body t3 ->
+      red t1 t1' ->
+      red (trm_match t1 c t2 t3) (trm_match t1' c t2 t3)
+  | red_match_2 : forall c t1 t2 t3,
+      value (trm_constructor c t1) ->
+      term_body t2 ->
+      term_body t3 ->
+      red (trm_match (trm_constructor c t1) c t2 t3) (t2 ^^ t1)
+  | red_match_3 : forall c d t1 t2 t3,
+      c <> d ->
+      value (trm_constructor d t1) ->
+      term_body t2 ->
+      term_body t3 ->
+      red (trm_match (trm_constructor d t1) c t2 t3)
+          (t3 ^^ (trm_constructor d t1))
+  | red_absurd : forall t1 t1',
+      red t1 t1' ->
+      red (trm_absurd t1) (trm_absurd t1').
+                  
+Notation "t --> t'" := (red t t') (at level 68).
+
+(* ************************************************************** *)
+(** ** Description of the results *)
+
+(** Goal is to prove preservation and progress *)
+
+Definition preservation := forall E t t' T,
+  E |= t -: T ->
+  t --> t' ->
+  E |= t' -: T.
+
+
+Definition progress := forall t T, 
+  empty |= t -: T ->
+     value t 
+  \/ exists t', t --> t'.
