Infrastructure.v
@@ -1,0 +1,1131 @@
+(************************************************
+ *          Row Subtyping - Infrastructure      *
+ *                 Leo White                    *
+ ************************************************)
+
+Set Implicit Arguments.
+Require Import List LibLN Definitions.
+
+
+(* =============================================================== *)
+(** * Additional Definitions used in the Proofs *)
+
+(* *************************************************************** *)
+(** ** Free Variables *)
+
+(** Computing free variables of a type. *)
+
+Fixpoint typ_fv (T : typ) {struct T} : vars :=
+  match T with
+  | typ_bvar i => \{}
+  | typ_fvar x => \{x}
+  | typ_constructor c T1 => (typ_fv T1)
+  | typ_variant T1 T2 => (typ_fv T1) \u (typ_fv T2)
+  | typ_arrow T1 T2 => (typ_fv T1) \u (typ_fv T2)
+  | typ_top => \{}
+  | typ_bot => \{}
+  | typ_meet T1 T2 => (typ_fv T1) \u (typ_fv T2)
+  | typ_join T1 T2 => (typ_fv T1) \u (typ_fv T2)
+  end.
+
+(** Computing free variables of a list of terms. *)
+
+Definition typ_fv_list :=
+  fold_right (fun t acc => typ_fv t \u acc) \{}.
+
+(** Computing free variables of a type scheme. *)
+
+Definition sch_fv M := 
+  typ_fv (sch_type M).
+
+(** Computing free type variables of the values of an environment. *)
+
+Definition bind_fv (B : bind) : vars :=
+  match B with
+  | bind_kind K => \{}
+  | bind_typ M => sch_fv M
+  end.
+
+Definition env_fv := 
+  fv_in_values bind_fv.
+
+(** Computing free variables of a term. *)
+
+Fixpoint trm_fv (t : trm) {struct t} : vars :=
+  match t with
+  | trm_bvar i => \{}
+  | trm_fvar x => \{x}
+  | trm_abs t1 => trm_fv t1
+  | trm_let t1 t2 => (trm_fv t1) \u (trm_fv t2)
+  | trm_app t1 t2 => (trm_fv t1) \u (trm_fv t2)
+  | trm_constructor c t1 => trm_fv t1
+  | trm_match t1 c t2 t3 => (trm_fv t1) \u (trm_fv t2) \u (trm_fv t3)
+  | trm_absurd t1 => trm_fv t1
+  end.
+
+(* *************************************************************** *)
+(** ** Substitution for free names *)
+
+(** Substitution for names for types *)
+
+Fixpoint typ_subst (Z : var) (U : typ) (T : typ) {struct T} : typ :=
+  match T with
+  | typ_bvar i => typ_bvar i
+  | typ_fvar X => If X = Z then U else (typ_fvar X)
+  | typ_constructor c T1 => typ_constructor c (typ_subst Z U T1)
+  | typ_variant T1 T2 =>
+      typ_variant (typ_subst Z U T1) (typ_subst Z U T2)
+  | typ_arrow T1 T2 =>
+      typ_arrow (typ_subst Z U T1) (typ_subst Z U T2)
+  | typ_top => typ_top
+  | typ_bot => typ_bot
+  | typ_meet T1 T2 =>
+      typ_meet (typ_subst Z U T1) (typ_subst Z U T2)
+  | typ_join T1 T2 =>
+      typ_join (typ_subst Z U T1) (typ_subst Z U T2)
+  end.
+
+(** Iterated substitution for types  *)
+
+Fixpoint typ_substs (Zs : list var) (Us : list typ) (T : typ)
+   {struct Zs} : typ :=
+  match Zs, Us with
+  | Z::Zs', U::Us' => typ_substs Zs' Us' (typ_subst Z U T)
+  | _, _ => T
+  end.    
+
+(** Substitution for names for schemes. *)
+
+Definition sch_subst Z U M := 
+  Sch (sch_kinds M) (typ_subst Z U (sch_type M)).
+
+(** Iterated substitution for schemes. *)
+
+Definition sch_substs Zs Us M := 
+  Sch (sch_kinds M) (typ_substs Zs Us (sch_type M)).
+
+(** Substitution for bindings *)
+Definition binding_subst Z U B :=
+  match B with
+  | bind_kind K => bind_kind K
+  | bind_typ M => bind_typ (sch_subst Z U M)
+  end.
+
+Definition environment_subst Z U E :=
+  map (binding_subst Z U) E.
+
+Fixpoint environment_substs (Zs : list var) (Us : list typ) (E : env)
+   {struct Zs} : env :=
+  match Zs, Us with
+  | Z::Zs', U::Us' => environment_substs Zs' Us' (environment_subst Z U E)
+  | _, _ => E
+  end.    
+
+(** Substitution for name in a term. *)
+
+Fixpoint trm_subst (z : var) (u : trm) (t : trm) {struct t} : trm :=
+  match t with
+  | trm_bvar i => trm_bvar i 
+  | trm_fvar x => If x = z then u else (trm_fvar x)
+  | trm_abs t1 => trm_abs (trm_subst z u t1) 
+  | trm_let t1 t2 => trm_let (trm_subst z u t1) (trm_subst z u t2) 
+  | trm_app t1 t2 => trm_app (trm_subst z u t1) (trm_subst z u t2)
+  | trm_constructor c t1 => trm_constructor c (trm_subst z u t1)
+  | trm_match t1 c t2 t3 =>
+      trm_match (trm_subst z u t1) c
+                (trm_subst z u t2) (trm_subst z u t3)
+  | trm_absurd t1 => trm_absurd (trm_subst z u t1)
+  end.
+
+Notation "[ z ~> u ] t" := (trm_subst z u t) (at level 68).
+
+(* =============================================================== *)
+(** * Tactics *)
+
+(* *************************************************************** *)
+(** ** Instanciation of Tactics *)
+
+Ltac gather_vars :=
+  let A := gather_vars_with (fun x : vars => x) in
+  let B := gather_vars_with (fun x : var => \{x}) in
+  let C := gather_vars_with (fun x : env => dom x) in
+  let D := gather_vars_with (fun x : LibEnv.env bind => dom x) in
+  let E := gather_vars_with (fun x : trm => trm_fv x) in
+  let F := gather_vars_with (fun x : typ => typ_fv x) in
+  let G := gather_vars_with (fun x : list typ => typ_fv_list x) in
+  let H := gather_vars_with (fun x : env => env_fv x) in
+  let I := gather_vars_with (fun x : LibEnv.env bind => env_fv x) in
+  let J := gather_vars_with (fun x : sch => sch_fv x) in
+  constr:(A \u B \u C \u D \u E \u F \u G \u H \u I \u J).
+
+Tactic Notation "pick_fresh" ident(x) :=
+  let L := gather_vars in (pick_fresh_gen L x).
+
+Tactic Notation "pick_freshes" constr(n) ident(x) :=
+  let L := gather_vars in (pick_freshes_gen L n x).
+
+Tactic Notation "apply_fresh" constr(T) "as" ident(x) :=
+  apply_fresh_base T gather_vars x.
+
+Tactic Notation "apply_fresh" "*" constr(T) "as" ident(x) :=
+  apply_fresh T as x; autos*.
+
+Tactic Notation "exists_fresh" ident(x) ident(Hfr) :=
+  exists_fresh_gen gather_vars x Hfr.
+
+(* *************************************************************** *)
+(** ** Automation *)
+
+Hint Constructors type term environment type_equal kinding kinding_env typing value red.
+
+Lemma typ_def_fresh : typ_fv typ_def = \{}.
+Proof.
+  easy.
+Qed.
+
+Hint Extern 1 (_ \notin typ_fv typ_def) =>
+  rewrite typ_def_fresh.
+
+Hint Extern 1 (types _ _) => split; auto.
+
+Hint Extern 1 =>
+  match goal with
+  | H : forall x, x \notin ?L -> ?P |- ?P =>
+    apply (H (proj1_sig (var_fresh L)) (proj2_sig (var_fresh L)))
+  | H: forall Xs : list var,
+      fresh ?L ?n Xs -> ?P |- ?P =>
+    apply (H (proj1_sig (var_freshes L n))
+             (proj2_sig (var_freshes L n)))
+  end.
+
+Lemma kinds_nil : forall E,
+    E & nil ~::* nil = E.
+Proof.    
+  intro.
+  rewrite singles_nil.
+  rewrite map_empty.
+  rewrite concat_empty_r.
+  auto.
+Qed.
+
+Lemma kinds_cons : forall E X Xs K Ks,
+    E & (X :: Xs) ~::* (K :: Ks) = E & Xs ~::* Ks & X ~:: K.
+Proof.    
+  intros.
+  rewrite singles_cons.
+  rewrite map_push.
+  rewrite concat_assoc.
+  auto.
+Qed.
+
+Hint Rewrite kinds_nil : rew_kinds.
+Hint Rewrite kinds_cons : rew_kinds.
+
+Tactic Notation "rew_kinds" :=
+  autorewrite with rew_kinds.
+
+Tactic Notation "rew_kinds" "*" :=
+  autorewrite with rew_kinds; auto.
+
+Tactic Notation "rew_kinds" "in" hyp(H) :=
+  autorewrite with rew_kinds in H.
+
+Tactic Notation "rew_kinds" "*" "in" hyp(H) :=
+  autorewrite with rew_kinds in H; auto.
+
+(* =============================================================== *)
+(** ** Properties of fv *)
+
+Lemma fv_list_map : forall ts1 ts2,
+  typ_fv_list (ts1 ++ ts2) = typ_fv_list ts1 \u typ_fv_list ts2.
+Proof.
+  induction ts1; simpl; intros. 
+  - rewrite* union_empty_l.
+  - rewrite IHts1.
+    rewrite* union_assoc.
+Qed.
+
+(* =============================================================== *)
+(** * Properties of terms *)
+
+(** Substitution on indices is identity on well-formed terms. *)
+
+Lemma trm_open_rec_core :forall t j v i u, i <> j ->
+  {j ~> v}t = {i ~> u}({j ~> v}t) -> t = {i ~> u}t.
+Proof.
+  induction t; introv Neq Equ;
+    simpl in *; inversion* Equ; f_equal*.
+  case_nat*. case_nat*.
+Qed.
+
+Lemma trm_open_rec : forall t u,
+  term t -> forall k, t = {k ~> u}t.
+Proof.
+  induction 1; intros; simpl; f_equal*. 
+  { unfolds trm_open. pick_fresh x.
+   apply* (@trm_open_rec_core t1 0 (trm_fvar x)). }
+  { unfolds trm_open. pick_fresh x.
+    apply* (@trm_open_rec_core t2 0 (trm_fvar x)). }
+  { unfolds trm_open. pick_fresh x.
+    apply* (@trm_open_rec_core t2 0 (trm_fvar x)). }
+  { unfolds trm_open. pick_fresh x.
+    apply* (@trm_open_rec_core t3 0 (trm_fvar x)). }
+Qed.
+
+(** Substitution for a fresh name is identity. *)
+
+Lemma trm_subst_fresh : forall x t u, 
+  x \notin trm_fv t ->  [x ~> u] t = t.
+Proof.
+  intros. induction t; simpls; f_equal*.
+  case_var*. 
+Qed.
+
+(** Substitution distributes on the open operation. *)
+
+Lemma trm_subst_open : forall x u t1 t2, term u -> 
+  [x ~> u] (t1 ^^ t2) = ([x ~> u]t1) ^^ ([x ~> u]t2).
+Proof.
+  intros. unfold trm_open. generalize 0.
+  induction t1; intros; simpl; f_equal*.
+  case_nat*. case_var*. apply* trm_open_rec.
+Qed.
+
+(** Substitution and open_var for distinct names commute. *)
+
+Lemma trm_subst_open_var : forall x y u e, y <> x -> term u ->
+  ([x ~> u]e) ^ y = [x ~> u] (e ^ y).
+Proof.
+  introv Neq Wu. rewrite* trm_subst_open.
+  simpl. case_var*.
+Qed.
+
+(** Opening up an abstraction of body t with a term u is the same as
+  opening up the abstraction with a fresh name x and then substituting u
+  for x. *)
+
+Lemma trm_subst_intro : forall x t u, 
+  x \notin (trm_fv t) -> term u ->
+  t ^^ u = [x ~> u](t ^ x).
+Proof.
+  introv Fr Wu. rewrite* trm_subst_open.
+  rewrite* trm_subst_fresh. simpl. case_var*.
+Qed.
+
+(** Terms are stable by substitution *)
+
+Lemma trm_subst_term : forall t z u,
+  term u -> term t -> term ([z ~> u]t).
+Proof.
+  induction 2; simpls*.
+  - case_var*.
+  - apply_fresh term_abs as y. rewrite* trm_subst_open_var.
+  - apply_fresh* term_let as y. rewrite* trm_subst_open_var.
+  - apply_fresh* term_match as y; rewrite* trm_subst_open_var.
+Qed.
+
+Hint Resolve trm_subst_term.
+
+(** Conversion from locally closed abstractions and bodies *)
+
+Lemma term_abs_to_body : forall t1, 
+  term (trm_abs t1) -> term_body t1.
+Proof.
+  intros. unfold term_body. inversion* H.
+Qed.
+
+Lemma body_to_term_abs : forall t1, 
+  term_body t1 -> term (trm_abs t1).
+Proof.
+  intros. inversion* H.
+Qed.
+
+Lemma term_let_to_body : forall t1 t2, 
+  term (trm_let t1 t2) -> term_body t2.
+Proof.
+  intros. unfold term_body. inversion* H.
+Qed.
+
+Lemma body_to_term_let : forall t1 t2, 
+  term_body t2 -> term t1 -> term (trm_let t1 t2).
+Proof.
+  intros. inversion* H.
+Qed.
+
+Lemma term_match_to_body1 : forall c t1 t2 t3,
+  term (trm_match t1 c t2 t3) -> term_body t2.
+Proof.
+  intros. unfold term_body. inversion* H.
+Qed.
+
+Lemma term_match_to_body2 : forall c t1 t2 t3,
+  term (trm_match t1 c t2 t3) -> term_body t3.
+Proof.
+  intros. unfold term_body. inversion* H.
+Qed.
+
+Lemma bodies_to_term_match : forall c t1 t2 t3,
+  term t1 -> term_body t2 -> term_body t3 ->
+  term (trm_match t1 c t2 t3).
+Proof.
+  intros. inversion H0. inversion H1.
+  apply* (@term_match (x \u x0)).
+Qed.
+
+Hint Resolve body_to_term_abs body_to_term_let bodies_to_term_match.
+
+Hint Extern 1 (term_body ?t) =>
+  match goal with 
+  | H: context [trm_abs t] |- _ => 
+    apply term_abs_to_body 
+  | H: context [trm_let ?t1 t] |- _ => 
+    apply (@term_let_to_body t1) 
+  | H: context [trm_match ?t1 ?c t ?t3] |- _ => 
+    apply (@term_match_to_body1 c t1 t t3) 
+  | H: context [trm_match ?t1 ?c ?t2 t] |- _ => 
+    apply (@term_match_to_body2 c t1 t2 t)
+  end.
+
+(** ** Opening a body with a term gives a term *)
+
+Lemma trm_open_term : forall t u,
+  term_body t -> term u -> term (t ^^ u).
+Proof.
+  intros. destruct H. pick_fresh y. rewrite* (@trm_subst_intro y).
+Qed.
+
+Hint Resolve trm_open_term.
+
+(* =============================================================== *)
+(** * Properties of types *)
+
+(** Open on a type is the identity. *)
+
+Lemma typ_open_type : forall T Us,
+  type T -> T = typ_open T Us.
+Proof.
+  introv W. induction T; simpls; inversions W; f_equal*.
+Qed.
+
+(** Substitution for a fresh name is identity. *)
+
+Lemma typ_subst_fresh : forall X U T, 
+  X \notin typ_fv T -> 
+  typ_subst X U T = T.
+Proof.
+  intros. induction T; simpls; f_equal*. case_var*. 
+Qed.
+
+Lemma typ_subst_fresh_list : forall z u ts,
+  z \notin typ_fv_list ts ->
+  ts = List.map (typ_subst z u) ts.
+Proof.
+  induction ts; simpl; intros Fr.
+  - easy.
+  -
+    f_equal*.
+    rewrite~ typ_subst_fresh.
+Qed.
+
+Lemma typ_subst_fresh_trm_fvars : forall z u xs,
+  fresh (\{z}) (length xs) xs ->
+  typ_fvars xs = List.map (typ_subst z u) (typ_fvars xs).
+Proof.
+  intros. apply typ_subst_fresh_list.
+  induction xs; simpl.
+  - auto.
+  - destruct H. auto.
+Qed.
+
+Lemma typ_substs_fresh : forall xs us t, 
+  fresh (typ_fv t) (length xs) xs -> 
+  typ_substs xs us t = t.
+Proof.
+  induction xs; simpl; intros us t Fr.
+  easy. destruct us. easy.
+  inversions Fr. rewrite* typ_subst_fresh.
+Qed.
+
+(** Substitution distributes on the open operation. *)
+
+Lemma typ_subst_open : forall X U T1 T2, type U -> 
+  typ_subst X U (typ_open T1 T2) = 
+   typ_open (typ_subst X U T1) (List.map (typ_subst X U) T2).
+Proof.
+  intros. induction T1; intros; simpl; f_equal*.
+  - symmetry. apply map_nth with (f := typ_subst X U) (d := typ_def). 
+  - case_var*. apply* typ_open_type.
+Qed.
+
+(** Substitution and open_var for distinct names commute. *)
+
+Lemma typ_subst_open_vars : forall X Ys U T, 
+  fresh \{X} (length Ys) Ys -> 
+  type U ->
+     typ_open_vars (typ_subst X U T) Ys
+   = typ_subst X U (typ_open_vars T Ys).
+Proof.
+  introv Fr Tu. unfold typ_open_vars.
+  rewrite* typ_subst_open. f_equal.
+  induction Ys; simpls.
+  - easy.
+  - destruct Fr.
+    case_var. f_equal*.
+Qed.
+
+Lemma app_last : forall A (x : A) l1 l2,
+  l1 ++ (x::l2) = (l1 ++(x :: nil)) ++ l2.
+Proof.
+  intros.
+  rewrite <- app_assoc.
+  easy.
+Qed.
+
+Lemma forall_app : forall A (l1 : list A) (l2 : list A) P,
+    Forall P l1 -> Forall P l2 -> Forall P (l1 ++ l2).
+Proof.
+  introv H1 H2.
+  induction* H1.
+  apply* Forall_cons.
+Qed.
+
+(** Opening up an abstraction of body t with a term u is the same as
+  opening up the abstraction with a fresh name x and then substituting u
+  for x. *)
+
+Lemma typ_substs_intro_ind : forall T Xs Us Vs, 
+  fresh (typ_fv T \u typ_fv_list Vs \u typ_fv_list Us) (length Xs) Xs -> 
+  types (length Xs) Us ->
+  types (length Vs) Vs ->
+  typ_open T (Vs ++ Us) =
+  typ_substs Xs Us (typ_open T (Vs ++ (typ_fvars Xs))).
+Proof.
+  induction Xs; simpl; introv Fr Tu Tv;
+   destruct Tu; destruct Us; tryfalse; auto.
+  inversions H0. lets [Fr1 Fr2]: Fr. simpls.
+  rewrite app_last.
+  forwards K: (IHXs Us (Vs ++ (t :: nil))); clear IHXs; auto.
+    { rewrite* fv_list_map. }
+    { split~. apply forall_app.
+      - lets* [_ Tv2] : Tv.
+      - auto. }
+  rewrite K. clear K. 
+  f_equal. rewrite~ typ_subst_open. rewrite~ typ_subst_fresh.
+  f_equal. rewrite map_app.
+  simpl. case_var; tryfalse*.
+  rewrite <- app_last. 
+  f_equal.
+  - apply~ typ_subst_fresh_list.
+  - f_equal. apply* typ_subst_fresh_trm_fvars.
+Qed.
+
+Lemma typ_substs_intro : forall Xs Us T, 
+  fresh (typ_fv T \u typ_fv_list Us) (length Xs) Xs -> 
+  types (length Xs) Us ->
+  (typ_open T Us) = typ_substs Xs Us (typ_open_vars T Xs).
+Proof.
+  intros. apply* (@typ_substs_intro_ind T Xs Us nil).
+Qed.
+
+(** Types are stable by type substitution *)
+
+Lemma typ_subst_type : forall T Z U,
+  type U -> type T -> type (typ_subst Z U T).
+Proof.
+  induction 2; simpls*. case_var*.
+Qed.
+
+Hint Resolve typ_subst_type.
+
+(** Types are stable by iterated type substitution *)
+
+Lemma typ_substs_types : forall Xs Us T,
+  types (length Xs) Us ->
+  type T ->
+  type (typ_substs Xs Us T).
+Proof.
+  induction Xs; destruct Us; simpl; introv TU TT; auto.
+  destruct TU. simpls. inversions H. inversions* H0.
+Qed.
+
+(** List of types are stable by type substitution *)
+
+Lemma typ_subst_type_list : forall Z U Ts n,
+  type U -> types n Ts -> 
+  types n (List.map (typ_subst Z U) Ts).
+Proof.
+  unfold types, list_for_n.
+  induction Ts; destruct n; simpl; intros TU [EQ TT]. 
+  easy. easy. inversion EQ.
+  inversions TT. forwards*: (IHTs n).
+Qed.
+
+(** ** Opening a body with a list of types gives a type *)
+
+Lemma fresh_length : forall L n xs,
+  fresh L n xs -> n = length xs.
+Proof using.
+  intros. gen n L. induction xs; simpl; intros n L Fr;
+    destruct n; tryfalse*.
+  easy.
+  f_equal.
+  rewrite* <- (@IHxs n (L \u \{a})).
+Qed.
+
+Lemma typ_open_types : forall n T Us,
+  type_body n T ->
+  types n Us -> 
+  type (typ_open T Us).
+Proof. 
+  introv [L K] H. pick_freshes n Xs.
+  lets Fr': Fr.
+  rewrite (fresh_length _ _ _ Fr)  in H, Fr'.
+  rewrite* (@typ_substs_intro Xs). apply* typ_substs_types.
+Qed.
+
+(* =============================================================== *)
+(** * Properties of schemes *)
+
+(** Substitution for a fresh name is identity. *)
+
+Lemma sch_subst_fresh : forall X U M, 
+  X \notin sch_fv M -> 
+  sch_subst X U M = M.
+Proof.
+  intros. destruct M as [n T]. unfold sch_subst.
+  rewrite* typ_subst_fresh.
+Qed.
+
+(** Trivial lemma to unfolding definition of [sch_subst] by rewriting. *)
+
+Lemma sch_subst_fold : forall Z U T Ks,
+  Sch Ks (typ_subst Z U T) = sch_subst Z U (Sch Ks T).
+Proof.
+  easy.
+Qed. 
+
+(** Distributivity of type substitution on opening of scheme. *)
+
+Lemma sch_subst_open : forall Z U M Us,
+   type U ->
+    typ_subst Z U (sch_open M Us)
+  = sch_open (sch_subst Z U M) (List.map (typ_subst Z U) Us).
+Proof.
+  unfold sch_open. intros. destruct M. simpl.
+  rewrite* <- typ_subst_open.
+Qed.
+
+(** Distributivity of type substitution on opening of scheme with variables. *)
+
+Lemma sch_subst_open_vars : forall Z U M Xs,
+   fresh (\{Z}) (length Xs) Xs -> 
+   type U ->
+    typ_subst Z U (sch_open_vars M Xs)
+  = sch_open_vars (sch_subst Z U M) Xs.
+Proof.
+  unfold sch_open_vars. intros. destruct M.
+  rewrite* <- typ_subst_open_vars.
+Qed.
+
+(** Schemes are stable by type substitution. *)
+
+Lemma sch_subst_type : forall Z U M,
+  type U -> scheme M -> scheme (sch_subst Z U M).
+Proof.
+  unfold scheme, sch_subst, sch_arity.
+  intros Z U [Ks T] TU S.
+  simpls.
+  destruct S as [L H].
+  exists_fresh Xs Fr.
+  rewrite* typ_subst_open_vars.
+  rewrite* (fresh_length _ _ _ Fr) in Fr.
+Qed.
+
+Hint Resolve sch_subst_type.
+
+(** Scheme arity is preserved by type substitution. *)
+
+Lemma sch_subst_arity : forall X U M, 
+  sch_arity (sch_subst X U M) = sch_arity M.
+Proof.
+  easy.
+Qed.
+
+(** ** Opening a scheme with a list of types gives a type *)
+
+Lemma sch_open_types : forall M Us,
+  scheme M ->
+  types (sch_arity M) Us ->
+  type (sch_open M Us).
+Proof.
+  intros [Ks T] Us Hb [Ha Ht].
+  simpls. apply* typ_open_types.
+Qed.
+
+Hint Resolve sch_open_types.
+
+(* =============================================================== *)
+(** * Properties of environment *)
+
+Lemma environment_typ_push_inv : forall E x M,
+    environment (E & x ~ (bind_typ M)) ->
+    environment E /\ x # E /\ scheme M.
+Proof.
+  introv H.
+  inverts H as H1 H2 H3 H4.
+  - false (empty_push_inv H1).
+  - destruct (eq_push_inv H3) as [_ [Hv _]].
+    false Hv.
+  - destruct (eq_push_inv H4) as [Hx [Hv He]].
+    inversion Hv.
+    subst.
+    easy.
+Qed.
+
+Lemma environment_kind_push_inv : forall E x K,
+    environment (E & x ~ (bind_kind K)) ->
+    environment E /\ x # E.
+Proof.
+  introv H.
+  inverts H as H1 H2 H3 H4.
+  - false (empty_push_inv H1).
+  - destruct (eq_push_inv H3) as [Hx [_ He]].
+    subst.
+    easy.
+  - destruct (eq_push_inv H4) as [_ [Hv _]].
+    false Hv.
+Qed.
+
+Lemma environment_typ_middle_inv : forall E x M F,
+    environment (E & x ~ (bind_typ M) & F) ->
+    environment (E & F) /\ x # E /\ scheme M.
+Proof.
+  introv H.
+  induction F using env_ind; rew_env_concat.
+  - rewrite concat_empty_r in H.
+    destruct* (environment_typ_push_inv H).
+  - rewrite concat_assoc in H.
+    destruct v.
+    + destruct* (environment_kind_push_inv H).
+    + destruct* (environment_typ_push_inv H).
+Qed.
+
+Lemma environment_kind_middle_inv : forall E x K F,
+    environment (E & x ~ (bind_kind K) & F) ->
+    environment (E & F) /\ x # E.
+Proof.
+  introv H.
+  induction F using env_ind; rew_env_concat.
+  - rewrite concat_empty_r in H.
+    destruct* (environment_kind_push_inv H).
+  - rewrite concat_assoc in H.
+    destruct v.
+    + destruct* (environment_kind_push_inv H).
+    + destruct* (environment_typ_push_inv H).
+Qed.
+
+Lemma environment_concat_inv : forall E F G,
+    environment (E & F & G) -> environment (E & G).
+Proof.
+  intros E F G.
+  induction F using env_ind; rew_env_concat; auto.
+  intro H.
+  destruct v.
+  - destruct* (environment_kind_middle_inv H).
+  - destruct* (environment_typ_middle_inv H).
+Qed.
+
+Lemma environment_concat_inv_l : forall E F,
+  environment (E & F) ->
+  environment E.
+Proof.
+  introv H.
+  rewrite <- (concat_empty_r F) in H.
+  rewrite concat_assoc in H.
+  rewrite <- (concat_empty_r E).
+  apply (environment_concat_inv H).
+Qed.
+
+Lemma environment_concat_inv_r : forall E F,
+  environment (E & F) ->
+  environment F.
+Proof.
+  introv H.
+  rewrite <- (concat_empty_l E) in H.
+  rewrite <- (concat_empty_l F).
+  apply (environment_concat_inv H).
+Qed.
+
+Hint Extern 1 (environment ?E) =>
+  match goal with
+  | H: environment (E & _) |- _ =>
+      apply (environment_concat_inv_l H)
+  | H: environment (_ & E) |- _ =>
+      apply (environment_concat_inv_r H)
+  end.
+
+Lemma environment_subst_inv_r : forall E F X T,
+  environment (E & F) ->
+  type T ->
+  environment (E & environment_subst X T F).
+Proof.
+  introv He Ht.
+  unfold environment_subst.
+  induction F using env_ind;
+    rew_env_concat; autorewrite with rew_env_map; auto.
+  rewrite concat_assoc in *.
+  destruct v; simpl.
+  - destruct (environment_kind_push_inv He).
+    apply* environment_kind.
+  - destruct (environment_typ_push_inv He).
+    apply*  environment_typ.
+Qed.
+
+Lemma environment_subst_empty : forall X T,
+    environment_subst X T empty = empty.
+Proof.
+  intros.
+  unfold environment_subst.
+  rewrite map_empty.
+  auto.
+Qed.
+
+Lemma environment_substs_empty : forall Xs Ts,
+    length Xs = length Ts ->
+    environment_substs Xs Ts empty = empty.
+Proof.
+  introv Hl.
+  gen Ts.
+  induction Xs.
+  - induction Ts; introv Hl; tryfalse; auto.
+  - induction Ts; introv Hl; tryfalse.
+    simpl.
+    rewrite environment_subst_empty.
+    auto.
+Qed.
+
+Lemma fresh_kinds : forall E x n Xs Ks,
+    fresh (dom E) (S n) (x :: Xs) ->
+    length Xs = length Ks ->
+    x # (E & Xs ~::* Ks).
+Proof.
+  introv Hf.
+  destruct Hf as [Hu Hx].
+  rewrite dom_concat.
+  rewrite notin_union.
+  split*.
+  rewrite dom_map.
+  rewrite dom_singles.
+  - eapply fresh_single_notin.
+    eapply fresh_union_r2.
+    apply Hx.
+  - { clear Hx.
+      gen Ks.
+      - induction Xs.
+        + induction Ks; intros; tryfalse; auto.
+        + induction Ks; intros; tryfalse.
+          rewrite! LibList.length_cons.
+          f_equal*. }
+Qed.
+
+Lemma environment_kinds : forall E n Xs Ks,
+    environment E ->
+    (fresh (dom E) n Xs) ->
+    length Ks = n ->
+    environment (E & Xs ~::* Ks).
+Proof.
+  introv He Hf Hlk.
+  lets Hlx : (eq_sym (fresh_length _ _ _ Hf)).
+  gen Ks n.
+  induction Xs.
+  - induction Ks; intros; subst; tryfalse.
+    rew_kinds*.
+  - induction Ks; intros; subst; tryfalse.
+    rew_kinds.
+    apply environment_kind.
+    + eapply IHXs; intuition.
+      destruct* Hf.
+    + eapply fresh_kinds; auto.
+Qed.
+
+(** Binding substitution is identity on bind_kind. *)
+
+Lemma binding_subst_kind : forall x T K,
+  binding_subst x T (bind_kind K) = bind_kind K.
+Proof.
+  simpl.
+  reflexivity.
+Qed.
+
+Lemma binds_subst_inv_r : forall E F X Y T K,
+    binds X (bind_kind K) (E & F) ->
+    binds X (bind_kind K) (E & environment_subst Y T F).
+Proof.
+  introv H.
+  unfolds environment_subst.
+  destruct (binds_concat_inv H).
+  - apply binds_concat_right.
+    erewrite <- binding_subst_kind .
+    apply* binds_map.
+  - apply* binds_concat_left.
+Qed.
+
+Hint Resolve binds_subst_inv_r.
+    
+Lemma ok_from_environment : forall E,
+  environment E -> ok E.
+Proof.
+  introv He.
+  induction He; auto. 
+Qed.
+
+Hint Resolve ok_from_environment.
+
+Lemma scheme_from_env : forall E x M,
+    environment E ->
+    binds x (bind_typ M) E ->
+    scheme M.
+Proof.
+  introv He Hb.
+  induction E using env_ind; rew_env_concat.
+  - false (binds_empty_inv Hb).
+  - destruct (binds_push_inv Hb)
+      as [ [ Hvar Hbind ] | [ Hvar Hbind ] ].
+    + { subst.
+        inversion He.
+        - false (empty_push_inv H0).
+        - destruct (eq_push_inv H) as [_ [Heq _]].
+          false Heq.
+        - destruct (eq_push_inv H) as [_ [Heq _]].
+          inversion Heq.
+          subst*. }
+    + eapply IHE; auto.
+Qed.
+
+(* =============================================================== *)
+(** * Properties of judgments *)
+
+(* *************************************************************** *)
+(** ** Regularity of relations *)
+
+(** A kinding relation is restricted to well-formed objects. *)
+
+Lemma kinding_regular : forall E T K,
+  kinding E T K -> environment E /\ type T.
+Proof.
+  split; induction* H.
+Qed.
+
+Lemma kindings_regular : forall E n Ts Ks,
+  kindings E n Ts Ks -> environment E /\ types n Ts.
+Proof.
+  split; induction* H.
+  split.
+  - simpl.
+    f_equal.
+    destruct* IHkindings.
+  - lets [_ Ht] : (kinding_regular H).
+    lets [_ Hts] : IHkindings.
+    apply* Forall_cons.
+Qed.  
+
+Lemma kinding_body_regular : forall E n Ks T,
+    kinding_body E n Ks T ->
+    environment E /\ type_body n T.
+Proof.
+  introv H.
+  destruct H as [L H].
+  split.
+  - pick_freshes n Xs.
+    eapply kinding_regular in H; auto.
+    destruct* H.
+  - exists_fresh Xs Hf.
+    eapply kinding_regular in H; auto.
+    destruct* H.
+Qed.
+
+Lemma kinding_scheme_regular : forall E M,
+    kinding_scheme E M -> environment E /\ scheme M.
+Proof.
+  introv H.
+  destruct (kinding_body_regular H).
+  split*.
+Qed.
+
+Lemma kinding_env_regular : forall E,
+    kinding_env E -> environment E.
+Proof.
+  introv H.
+  induction* H.
+  apply* environment_typ.
+  eapply proj2.
+  apply kinding_scheme_regular.
+  apply H0.
+Qed.
+
+(* Automation of kinding regularity lemmas *)
+
+Hint Extern 1 (type ?T) =>
+  match goal with
+  | H: kinding _ T _ |- _ =>
+      apply (proj2 (kinding_regular H))
+  end.
+
+Hint Extern 1 (scheme ?M) =>
+  match goal with
+  | H: kinding_scheme _ M |- _ =>
+      apply (proj2 (kinding_scheme_regular H))
+  | H1 : environment ?E, H2 : binds _ (bind_typ M) ?E |- _ =>
+      apply (scheme_from_env H1 H2)
+  | H1 : kinding_env ?E, H2 : binds _ (bind_typ M) ?E |- _ =>
+      apply (scheme_from_env (kinding_env_regular H1) H2)
+end.
+
+Hint Extern 1 (environment ?E) =>
+  match goal with
+  | H: kinding_env E |- _ =>
+      apply (kinding_env_regular H)
+  | H: kinding E _ _ |- _ =>
+      apply (proj1 (kinding_regular H))
+  | H: kindings E _ _ _ |- _ =>
+      apply (proj1 (kindings_regular H))
+  | H: kinding_body E _ _ _ |- _ =>
+      apply (proj1 (kinding_body_regular H))
+  | H: kinding_scheme E _ |- _ =>
+      apply (proj1 (kinding_scheme_regular H))
+  end.
+
+Hint Extern 1 (environment (?E & ?F)) =>
+  match goal with
+  | H: environment (E & _ & F) |- _ =>
+      apply (environment_concat_inv H)
+  end.
+
+Hint Extern 1 (types ?n ?Ts) =>
+  match goal with
+  | H: kindings _ n Ts _ |- _ =>
+      apply (proj2 (kindings_regular H))
+  end.
+
+Hint Extern 1 (type_body ?n ?T) =>
+  match goal with
+  | H: kinding_body _ n _ T |- _ =>
+      apply (proj2 (kinding_body_regular H))
+  end.
+
+(** Type equality preserves regularity *)
+
+Lemma type_equal_regular : forall E T1 T2 K,
+    type_equal E T1 T2 K -> environment E /\ type T1 /\ type T2.
+Proof.
+  introv Ht.
+  induction* Ht. 
+Qed.
+
+Lemma subtype_regular : forall E T1 T2,
+    subtype E T1 T2 -> environment E /\ type T1 /\ type T2.
+Proof.
+  introv Hs.
+  destruct (type_equal_regular Hs) as [ He [ _ Ht ] ].
+  inversion* Ht.
+Qed.
+
+(* Automation of equality regularity lemmas *)
+
+Hint Extern 1 (type ?T) =>
+  match goal with
+  | H: type_equal _ T _ _ |- _ =>
+      apply (proj32 (type_equal_regular H))
+  | H: type_equal _ _ T _ |- _ =>
+      apply (proj33 (type_equal_regular H))
+  | H: subtype _ T _ |- _ =>
+      apply (proj32 (subtype_regular H))
+  | H: subtype _ _ T |- _ =>
+      apply (proj33 (subtype_regular H))
+  end.
+
+Hint Extern 1 (environment ?E) =>
+  match goal with
+  | H: type_equal E _ _ _ |- _ =>
+      apply (proj31 (type_equal_regular H))
+  | H: subtype E _ _ |- _ =>
+      apply (proj31 (subtype_regular H))
+  end.
+
+Hint Extern 1 (environment (?E & environment_subst ?X ?T ?F)) =>
+  match goal with
+  | H1: environment (E & X ~:: ?K & F), H2: kinding E T ?K |- _ =>
+      apply (environment_subst_inv_r X
+               (environment_concat_inv H1)
+               (proj2 (kinding_regular H2)))
+  | H1: environment (E & X ~:: ?K & F), H2: type_equal E T T ?K |- _ =>
+      apply (environment_subst_inv_r X
+               (environment_concat_inv H1)
+               (proj31 (type_equal_regular H2)))
+  | H1: environment (E & X ~:: _ & F), H2: type T |- _ =>
+      apply (environment_subst_inv_r X (environment_concat_inv H1) H2)
+  | H1: environment (E & F), H2: type T |- _ =>
+      apply (environment_subst_inv_r X H1 H2)
+  end.
+
+(** A typing relation is restricted to well-formed objects. *)
+
+Lemma typing_regular : forall E e T,
+  typing E e T -> environment E /\ term e /\ type T.
+Proof.
+  splits 3.
+  - induction* H.
+    pick_freshes (sch_arity M) Xs.
+    eapply environment_concat_inv_l.
+    apply* H0.
+  - induction H; eauto.
+  - induction* H.
+    inversion* IHtyping1.
+Qed.
+
+(** Automation of typing regularity lemma *)
+
+Hint Extern 1 (environment ?E) =>
+  match goal with
+  | H: typing E _ _ |- _ =>
+      apply (proj31 (typing_regular H))
+  end.
+
+Hint Extern 1 (term ?e) =>
+  match goal with
+  | H: typing _ e _ |- _ =>
+      apply (proj32 (typing_regular H))
+  end.
+
+Hint Extern 1 (type ?T) =>
+  match goal with
+  | H: typing _ _ T |- _ =>
+      apply (proj33 (typing_regular H))
+  end.
+
+(** The value predicate is restricted to well-formed terms. *)
+
+Lemma value_regular : forall e,
+  value e -> term e.
+Proof.
+  introv Hv.
+  induction* Hv.
+Qed.
+
+Hint Resolve value_regular.
+
+(** A reduction relation is restricted to well-formed terms. *)
+
+Lemma red_regular : forall e e',
+  red e e' -> term e /\ term e'.
+Proof.
+  introv Hr.
+  induction* Hr.
+  inversion* H.    
+Qed.
+
+Hint Extern 1 (term ?t) =>
+  match goal with
+  | H: red t _ |- _ => apply (proj1 (red_regular H))
+  | H: red _ t |- _ => apply (proj2 (red_regular H))
+  end.
