Soundness.v
@@ -1,0 +1,623 @@
+(************************************************
+ *          Row Subtyping - Soundness           *
+ *                 Leo White                    *
+ ************************************************)
+
+Set Implicit Arguments.
+Require Import LibLN Definitions Infrastructure.
+
+(* *************************************************************** *)
+(** * Properties of kinding *)
+
+(* *************************************************************** *)
+(** Weakening *)
+
+Hint Resolve binds_weaken.
+
+Lemma kinding_weakening : forall E F G T K,
+   kinding (E & G) T K -> 
+   environment (E & F & G) ->
+   kinding (E & F & G) T K.
+Proof.
+  introv Hk He.
+  inductions Hk; auto.
+Qed.
+
+Hint Resolve kinding_weakening.
+
+Lemma kinding_weakening_l : forall E F T K,
+    kinding E T K ->
+    environment (E & F) ->
+    kinding (E & F) T K.
+Proof.
+  introv Hk He.
+  rewrite <- (concat_empty_r E) in Hk.
+  rewrite <- (concat_empty_r F) in *.
+  rewrite (concat_assoc E F empty) in *.
+  apply* kinding_weakening.
+Qed.
+
+Hint Resolve kinding_weakening_l.
+
+Lemma kinding_weakening_r : forall E F T K,
+    kinding E T K ->
+    environment (F & E) ->
+    kinding (F & E) T K.
+Proof.
+  introv Hk He.
+  rewrite <- (concat_empty_l E) in Hk.
+  rewrite <- (concat_empty_l F) in *.
+  apply* kinding_weakening.
+Qed.
+
+Hint Resolve kinding_weakening_r.
+
+Lemma kindings_weakening : forall E F G n Ts Ks,
+   kindings (E & G) n Ts Ks -> 
+   environment (E & F & G) ->
+   kindings (E & F & G) n Ts Ks.
+Proof.
+  introv Hk He.
+  gen_eq EG : (E & G).
+  induction Hk; intro; subst; auto.
+  - apply* kindings_nil.
+  - apply* kindings_cons.
+Qed.
+
+Hint Resolve kindings_weakening.
+
+Lemma kinding_body_weakening : forall E F G n Ks T,
+    kinding_body (E & G) n Ks T ->
+    length Ks = n ->
+    environment (E & F & G) ->
+    kinding_body (E & F & G) n Ks T.
+Proof.
+  unfold kinding_body.
+  introv Hk He.
+  destruct Hk as [L Hk].
+  exists_fresh Xs Hf.
+  apply_ih_bind* kinding_weakening.
+  apply environment_kinds with n; auto.
+  rewrite! dom_concat.
+  auto.
+Qed.  
+
+Hint Resolve kinding_body_weakening.
+
+Lemma kinding_scheme_weakening : forall E F G M,
+    kinding_scheme (E & G) M ->
+    environment (E & F & G) ->
+    kinding_scheme (E & F & G) M.
+Proof.
+  unfold kinding_scheme.
+  introv Hk He.
+  apply* kinding_body_weakening.
+Qed.
+
+Hint Resolve kinding_scheme_weakening.
+
+Lemma kinding_scheme_weakening_l : forall E F M,
+    kinding_scheme E M ->
+    environment (E & F) ->
+    kinding_scheme (E & F) M.
+Proof.
+  introv Hk He.
+  rewrite <- (concat_empty_r E) in Hk.
+  rewrite <- (concat_empty_r F) in *.
+  rewrite (concat_assoc E F empty) in *.
+  apply* kinding_scheme_weakening.
+Qed.  
+
+Hint Resolve kinding_scheme_weakening_l.
+
+(* *************************************************************** *)
+(** Not affected by type bindings *)
+
+Lemma kinding_bind_typ : forall E T K x S,
+    kinding (E & x ~: S) T K ->
+    kinding E T K.
+Proof.
+  introv Hk.
+  gen_eq Ex : (E & x ~: S).
+  induction Hk; intro; subst; eauto.
+  destruct* (binds_push_inv H0) as [ [ _ Heq ] | ].
+  inversion Heq.
+Qed.
+
+(* *************************************************************** *)
+(** Preserved by type substitution *)
+
+Lemma kinding_typ_subst : forall E F X T S K J,
+  kinding (E & X ~:: J & F) T K -> 
+  kinding E S J -> 
+  kinding (E & (environment_subst X S F)) (typ_subst X S T) K.
+Proof.
+  introv Hkt Hks.
+  gen_eq G : (E & X ~:: J & F).
+  induction Hkt; introv Heq; subst; simpl typ_subst; auto.
+  - case_var.
+    + lets Hb : (binds_middle_eq_inv H0 (ok_from_environment H)).
+      inversion Hb; subst.
+      apply* kinding_weakening_l.
+    + { apply* kinding_var.
+        - apply binds_subst_inv_r.
+          eapply binds_subst.
+          + apply H0.
+          + auto. }
+Qed.
+
+Lemma kinding_typ_subst_l : forall E X T S K J,
+  kinding (E & X ~:: J) T K -> 
+  kinding E S J -> 
+  kinding E (typ_subst X S T) K.
+Proof.
+  introv Hk1 Hk2.
+  rewrite <- concat_empty_r with (E := E).
+  rewrite <- environment_subst_empty with (X := X) (T := S).
+  apply kinding_typ_subst with (J := J); auto.
+  rewrite concat_empty_r.
+  auto.
+Qed.
+
+Lemma kinding_typ_substs : forall E F Xs T Ss K Js n,
+  kinding (E & Xs ~::* Js & F) T K -> 
+  kindings E n Ss Js -> 
+  length Xs = n ->
+  length Js = n ->
+  length Ss = n ->
+  kinding (E & (environment_substs Xs Ss F)) (typ_substs Xs Ss T) K.
+Proof.
+  intros.
+  gen Xs Ss Js T F.
+  induction n; introv Hlx Hls Hks Hlj Hkt; subst;
+    destruct Xs; destruct Ss; destruct Js; tryfalse; auto; simpl.
+  - rew_kinds* in Hkt.
+  - inversion Hlx.
+    inversion Hls.
+    inversion Hlj.
+    inversion Hks.
+    eapply IHn; eauto.
+    rew_kinds in Hkt.
+    eapply kinding_typ_subst.
+    + apply Hkt.
+    + apply* kinding_weakening_l.
+      eauto using environment_concat_inv_l.
+Qed.
+
+Lemma kinding_typ_substs_l : forall E Xs T Ss K Js n,
+  kinding (E & Xs ~::* Js) T K -> 
+  kindings E n Ss Js -> 
+  length Xs = n ->
+  length Js = n ->
+  length Ss = n ->
+  kinding E (typ_substs Xs Ss T) K.
+Proof.
+  introv Hk1 Hk2 Hlx Hlj Hls.
+  rewrite <- concat_empty_r with (E := E).
+  rewrite <- environment_substs_empty with (Xs := Xs) (Ts := Ss).
+  - apply kinding_typ_substs with (Js := Js) (n := n); auto.
+    rewrite concat_empty_r.
+    auto.
+  - subst*.
+Qed.
+
+Hint Resolve kinding_typ_subst.
+
+(* *************************************************************** *)
+(** Manipulating well-kinded environments *)
+
+Lemma kinding_env_shorten : forall E G,
+    kinding_env (E & G) ->
+    kinding_env E.
+Proof.
+  introv Hk.
+  induction G using env_ind;
+    autorewrite with rew_env_concat in Hk; auto.
+  inversion Hk.
+  - destruct (empty_concat_inv H0) as [ He1 _ ].
+    destruct (empty_concat_inv He1) as [ He2 _ ].
+    rewrite* <- He2.
+  - destruct (eq_push_inv H) as [ _ [ _ He ] ].
+    subst*.
+  - destruct (eq_push_inv H) as [ _ [ _ He ] ].
+    subst*.
+Qed.
+
+Hint Resolve kinding_env_shorten.
+
+Lemma kinding_env_kinds : forall E n Ks Xs,
+    kinding_env E ->
+    (fresh (dom E) n Xs) ->
+    length Ks = n ->
+    kinding_env (E & Xs ~::* Ks).
+Proof.
+  introv Hk Hf Hlk.
+  lets Hlx : (eq_sym (fresh_length _ _ _ Hf)).
+  gen Ks n.
+  induction Xs.
+  - induction Ks; intros; subst; tryfalse.
+    rew_kinds*.
+  - induction Ks; intros; subst; tryfalse.
+    rew_kinds.
+    apply kinding_env_kind.
+    + eapply IHXs; intuition.
+      destruct* Hf.
+    + eapply fresh_kinds; auto.
+Qed.
+
+Hint Resolve kinding_env_kinds.
+
+Lemma kinding_scheme_from_env : forall E x M,
+    kinding_env E ->
+    binds x (bind_typ M) E ->
+    kinding_scheme E M.
+Proof.
+  introv He Hb.
+  induction E using env_ind; rew_env_concat.
+  - false (binds_empty_inv Hb).
+  - destruct (binds_push_inv Hb)
+      as [ [ Hvar Hbind ] | [ Hvar Hbind ] ].
+    + { subst.
+        inversion He.
+        - false (empty_push_inv H0).
+        - destruct (eq_push_inv H) as [_ [Heq _]].
+          false Heq.
+        - destruct (eq_push_inv H) as [_ [Heq _]].
+          inversion Heq.
+          subst.
+          apply* kinding_scheme_weakening_l. }
+    + apply* kinding_scheme_weakening_l.
+Qed.
+
+Hint Resolve kinding_scheme_from_env.
+
+(* *************************************************************** *)
+(** Kinding of schemes with no parameters *)
+
+Lemma kinding_scheme_no_params : forall E T M,
+    kinding E T kind_type ->
+    M = Sch nil T ->
+    kinding_scheme E M.
+Proof.
+  introv Hk Heq.
+  subst.
+  exists_fresh Xs Hf.
+  simpl.
+  destruct (List.length_zero_iff_nil Xs) as [Hlz _].
+  rewrite (Hlz (eq_sym (fresh_length _ _ _ Hf))).
+  rewrite singles_nil.
+  rewrite map_empty.
+  rewrite concat_empty_r.
+  unfold typ_open_vars.
+  rewrite* <- (@typ_open_type T (typ_fvars nil)).
+Qed.
+
+Hint Resolve kinding_env_shorten.
+
+(* *************************************************************** *)
+(** * Properties of type equality *)
+
+(* *************************************************************** *)
+(** Reflexivity *)
+
+Lemma type_equal_refl : forall E T K,
+    kinding E T K ->
+    type_equal E T T K.
+Proof.
+  introv Hk.
+  induction* Hk.
+Qed.
+
+Hint Resolve type_equal_refl.
+
+(* *************************************************************** *)
+(** Symmetry *)
+
+Lemma type_equal_symm : forall E T1 T2 K,
+    type_equal E T1 T2 K ->
+    type_equal E T2 T1 K.
+Proof.
+  introv He.
+  induction* He.
+Qed.
+
+Hint Resolve type_equal_symm.
+
+(* *************************************************************** *)
+(** Idempotence of join and meet *)
+
+Lemma type_equal_join_idempotent : forall E T,
+    kinding E T kind_row ->
+    type_equal E (typ_join T T) T kind_row.
+Proof.
+  introv Hk.
+  apply type_equal_trans
+    with (typ_join T (typ_meet T typ_top)); auto.
+Qed.
+
+Hint Resolve type_equal_join_idempotent.
+
+Lemma type_equal_meet_idempotent : forall E T,
+    kinding E T kind_row ->
+    type_equal E (typ_meet T T) T kind_row.
+Proof.
+  introv Ht.
+  apply type_equal_trans
+    with (typ_meet T (typ_join T typ_bot)); auto.
+Qed.
+
+Hint Resolve type_equal_meet_idempotent.
+
+(* *************************************************************** *)
+(** Well-kindedness *)
+
+Lemma type_equal_kinding : forall E T1 T2 K,
+    type_equal E T1 T2 K ->
+    kinding E T1 K /\ kinding E T2 K.
+Proof.
+  introv He.
+  induction* He.
+Qed.
+
+Hint Extern 1 (kinding ?E ?T ?K) =>
+  match goal with
+  | H: type_equal E T _ K |- _ =>
+      apply (proj1 (type_equal_kinding H))
+  | H: type_equal E _ T K |- _ =>
+      apply (proj2 (type_equal_kinding H))
+  end.
+
+(* *************************************************************** *)
+(** Preserved by type substitution *)
+
+Lemma type_equal_typ_subst : forall E F X T1 T2 S K J,
+  type_equal (E & X ~:: J & F) T1 T2 K -> 
+  kinding E S J -> 
+  type_equal (E & (environment_subst X S F))
+             (typ_subst X S T1) (typ_subst X S T2) K.
+Proof.
+  introv Hkt Hks.
+  gen_eq G: (E & X ~:: J & F).
+  inductions Hkt; introv Heq; subst; simpl typ_subst; eauto.
+  - case_var.
+    + apply type_equal_refl.
+      lets Hb : (binds_middle_eq_inv H0 (ok_from_environment H)).
+      inversion Hb; subst.
+      apply* kinding_weakening_l.
+    + { apply* type_equal_var.
+        apply* binds_subst_inv_r.
+        eapply binds_subst.
+        - apply H0.
+        - auto. }
+Qed.
+
+Hint Resolve type_equal_typ_subst.
+
+(* *************************************************************** *)
+(** Weakening *)
+
+Lemma type_equal_weakening : forall E F G T1 T2 K,
+   type_equal (E & G) T1 T2 K -> 
+   environment (E & F & G) ->
+   type_equal (E & F & G) T1 T2 K.
+Proof.
+  introv Heq Henv.
+  inductions Heq; auto.
+  - apply type_equal_trans with T2.
+    + apply IHHeq1 with (E0 := E) (G0 := G); auto.
+    + apply IHHeq2 with (E0 := E) (G0 := G); auto.
+Qed.
+
+Hint Resolve type_equal_weakening.
+
+(* *************************************************************** *)
+(** * Properties of Subtyping *)
+
+(* *************************************************************** *)
+(** Reflexivity *)
+
+Lemma subtype_refl : forall E T,
+  kinding E T kind_row -> 
+  subtype E T T.
+Proof.
+  introv Hk.
+  inversion Hk; unfold subtype; auto.
+Qed.
+
+(* *************************************************************** *)
+(** Transitivity *)
+
+Lemma subtype_trans : forall E T1 T2 T3,
+    subtype E T1 T2 ->
+    subtype E T2 T3 ->
+    subtype E T1 T3.
+Proof.
+  introv H12 H23.
+  unfold subtype in *.
+  destruct (type_equal_kinding H23) as [ _ Hk ].
+  inversion Hk; subst.
+  apply type_equal_trans with (typ_join T1 T2); auto.
+  apply type_equal_trans with (typ_join T1 (typ_join T2 T3)); auto.
+  apply type_equal_trans with (typ_join (typ_join T1 T2) T3); auto.
+Qed.
+
+(* *************************************************************** *)
+(** Anti-symmetry *)
+
+Lemma subtype_antisymm : forall E T1 T2,
+    subtype E T1 T2 ->
+    subtype E T2 T1 ->
+    type_equal E T1 T2 kind_row.
+Proof.
+  introv H12 H21.
+  unfold subtype in *.
+  apply type_equal_trans with (typ_join T1 T2); auto.
+  apply type_equal_trans with (typ_join T2 T1); auto.
+Qed.
+
+(* *************************************************************** *)
+(* Well-kindedness *)
+
+Lemma subtype_kinding : forall E T1 T2,
+    subtype E T1 T2 ->
+    kinding E T1 kind_row /\ kinding E T2 kind_row.
+Proof.
+  introv He.
+  destruct (type_equal_kinding He) as [ Hk Hj ].
+  split*.
+  inversion* Hj.
+Qed.
+
+Hint Extern 1 (kinding ?E ?T kind_row) =>
+  match goal with
+  | H: subtype E T _ |- _ =>
+      apply (proj1 (subtype_kinding H))
+  | H: subtype E _ T |- _ =>
+      apply (proj2 (subtype_kinding H))
+  end.
+
+(* *************************************************************** *)
+(** Weakening *)
+
+Lemma subtype_weakening : forall E F G T1 T2,
+   subtype (E & G) T1 T2 -> 
+   environment (E & F & G) ->
+   subtype (E & F & G) T1 T2.
+Proof.
+  introv Hs He.
+  apply* type_equal_weakening.
+Qed.
+
+Hint Resolve subtype_weakening.
+
+(* *************************************************************** *)
+(** Preserved by type substitution *)
+
+Lemma subtype_typ_subst : forall E F X T1 T2 S J,
+  subtype (E & X ~:: J & F) T1 T2 -> 
+  kinding E S J -> 
+  subtype (E & (environment_subst X S F))
+          (typ_subst X S T1) (typ_subst X S T2).
+Proof.
+  unfold subtype.
+  introv Hs Hk.
+  lets H : (type_equal_typ_subst Hs Hk).
+  simpl in H.
+  auto.
+Qed.
+
+Hint Resolve subtype_typ_subst.
+
+(* *************************************************************** *)
+(** * Properties of typing *)
+
+Lemma typing_kinding_env : forall E e T,
+    typing E e T ->
+    kinding_env E.
+Proof.
+  introv Ht.
+  induction* Ht.
+  - pick_fresh x.
+    eapply kinding_env_shorten in H1; auto.
+  - pick_freshes (sch_arity M) Xs.
+    eapply kinding_env_shorten in H0; auto.
+Qed.
+
+Hint Resolve typing_kinding_env.
+
+Lemma typing_kinding : forall E e T,
+    typing E e T ->
+    kinding E T kind_type.
+Proof.
+  introv Ht.
+  induction* Ht.
+  - assert (kinding_scheme E M).
+    { apply kinding_scheme_from_env with x; auto. }
+    destruct H2 as [L Hs].
+    unfold sch_open.
+    pick_freshes (sch_arity M) Xs.
+    unfold sch_fv in Fr.
+    lets Hlx : (fresh_length _ _ _ Fr).
+    lets Hlk : (proj1 (proj2 (kindings_regular H1))).
+    apply kinding_typ_substs_l
+      with (Xs := Xs) (n := sch_arity M) (Ss := Us)
+      in Hs; auto.
+    rewrite (@typ_substs_intro Xs Us _); auto.
+    rewrite* <- Hlx.
+  - apply* kinding_arrow.
+    pick_fresh x.
+    eapply kinding_bind_typ in H1; auto.
+  - inversion* IHHt1.
+  - pick_fresh x.
+    eapply kinding_bind_typ in H2; auto.
+  - pick_fresh x.
+    eapply kinding_bind_typ in H0; auto.
+Qed.
+
+Hint Resolve typing_kinding.
+
+Lemma typing_scheme_kinding : forall E e M,
+    typing_scheme E e M ->
+    kinding_scheme E M.
+Proof.
+  introv [L Ht].
+  exists_fresh Xs Hf.
+  eapply typing_kinding in Ht; eauto.
+Qed.  
+
+Hint Resolve typing_scheme_kinding.
+
+(* *************************************************************** *)
+(** Weakening *)
+
+Lemma typing_weakening : forall E F G e T,
+   typing (E & G) e T -> 
+   kinding_env (E & F & G) ->
+   typing (E & F & G) e T.
+Proof.
+  introv Ht.
+  gen_eq EG : (E & G).
+  gen E F G.
+  induction Ht; intros; subst; eauto.
+  - apply_fresh* typing_abs as y.
+    apply_ih_bind H1; auto.
+    eapply kinding_scheme_no_params in H; auto.
+    apply* kinding_env_typ.
+  - apply_fresh (@typing_let M) as Ys.
+    + apply_ih_bind H0; auto.
+      apply kinding_env_kinds with (sch_arity M); auto.
+      rewrite! dom_concat.
+      auto.
+    + apply_ih_bind H2; auto.
+      apply* kinding_env_typ.
+      eapply typing_scheme_kinding.
+      exists_fresh Xs Hf.
+      apply_ih_bind H0; auto.
+      apply kinding_env_kinds with (sch_arity M); auto.
+      rewrite! dom_concat.
+      auto.
+  - apply_fresh* (@typing_match c) as Ys.
+    + { apply_ih_bind H0; auto.
+        apply* kinding_env_typ.
+        apply kinding_scheme_no_params with T3; auto.
+        assert (kinding (E0 & F & G)
+                  (typ_join (typ_constructor c T3) T6) kind_row)
+          by eauto.
+        inversion H6.
+        inversion H11.
+        auto. }
+    + apply_ih_bind H2; auto.
+      apply* kinding_env_typ.
+      apply kinding_scheme_no_params with (typ_variant T5 T6); auto.
+  - eapply typing_absurd; auto.
+Qed.
+   
+(* *************************************************************** *)
+(** Preserved by type substitution *)
+
+Lemma typing_typ_subst : forall F Z U E t T,
+  Z \notin (env_fv E) -> 
+  type U -> 
+  E & F |= t ~: T -> 
+  E & (map (sch_subst Z U) F) |= t ~: (typ_subst Z U T).
+
